Implement IP component and stack
Replace IPv4 with IPv6
Add more word conversion functions
Add IP subinterface to TCP component
Define TCP stack in terms of IP stack

TLC/IP.v
@@ -1,94 +1,181 @@
+Require Import Coq.Lists.List.
+Require Import Coq.Arith.EqNat.
+Require Import Coq.Arith.Minus.
+Require Import Coq.Arith.Plus.
+Require Import Coq.Numbers.Natural.Peano.NPeano.
+Require Import Coq.Vectors.Vector.
+Require Import TLC.Byte.
+Require Import TLC.Component.
+Require Import TLC.FairLossLink.
+Require Import TLC.Queue.
+Require Import TLC.Stack.
+Require Import TLC.TupleMap.
+Require Import TLC.Variant.
 Require Import TLC.Word.
+
+Import ListNotations.
 
 Set Implicit Arguments.
 Unset Strict Implicit.
 Unset Printing Implicit Defensive.
 
-Section ip.
+(* Primitives *)
+Definition ip_address := word 128.
+Definition ip_version := word 4.
+Definition ip_traffic_class := byte.
+Definition ip_flow_label := word 20.
+Definition ip_length := word 16.
+Definition ip_hop_limit := byte.
+Definition ip_payload := bytes.
 
-  Definition ip_address := word 32.
+(* Constants *)
+Definition ip_version_6 : ip_version := $6.
 
-  Inductive ip_precedence :=
-  | IpPrecedenceNetworkControl
-  | IpPrecedenceInternetworkControl
-  | IpPrecedenceCriticEcp
-  | IpPrecedenceFlashOverride
-  | IpPrecedenceFlash
-  | IpPrecedenceImmediate
-  | IpPrecedencePriority
-  | IpPrecedenceRoutine.
+(* Structures *)
+Inductive ip_next_header :=
+| IpNextHeaderTcp.
 
-  Definition ip_precedence_to_nat (p : ip_precedence) :=
-    match p with
-    | IpPrecedenceNetworkControl => 7
-    | IpPrecedenceInternetworkControl => 6
-    | IpPrecedenceCriticEcp => 5
-    | IpPrecedenceFlashOverride => 4
-    | IpPrecedenceFlash => 3
-    | IpPrecedenceImmediate => 2
-    | IpPrecedencePriority => 1
-    | IpPrecedenceRoutine => 0
-    end.
+Record ip_header :=
+  IpHeader {
+    ip_header_version : ip_version;
+    ip_header_traffic_class : ip_traffic_class;
+    ip_header_flow_label : ip_flow_label;
+    ip_header_payload_length : ip_length;
+    ip_header_next_header : ip_next_header;
+    ip_header_hop_limit : ip_hop_limit;
+    ip_header_src_address : ip_address;
+    ip_header_dst_address : ip_address;
+  }.
 
-  Definition ip_precedence_to_word (p : ip_precedence) : word 3 :=
-    natToWord _ (ip_precedence_to_nat p).
+Record ip_datagram :=
+  IpDatagram {
+    ip_datagram_header : ip_header;
+    ip_datagram_payload : ip_payload;
+  }.
 
-  Inductive ip_delay :=
-  | IpDelayNormal
-  | IpDelayLow.
+(* Encoders/decoders *)
+Definition ip_next_header_to_word (nh : ip_next_header) : byte :=
+  $match nh with
+  | IpNextHeaderTcp => 6
+  end.
 
-  Definition ip_delay_to_nat (d : ip_delay) :=
-    match d with
-    | IpDelayNormal => 0
-    | IpDelayLow => 1
-    end.
+Definition word_to_ip_next_header (w : byte) : option ip_next_header :=
+  if weqb w $6 then Some IpNextHeaderTcp
+  else None.
 
-  Definition ip_delay_to_word (d : ip_delay) : word 1 :=
-    natToWord _ (ip_delay_to_nat d).
+Definition ip_header_to_bytes (h : ip_header) : bytes :=
+  word64_to_bytes (
+    ip_header_version h ^::
+    ip_header_traffic_class h ^::
+    ip_header_flow_label h ^::
+    ip_header_payload_length h ^::
+    ip_next_header_to_word (ip_header_next_header h) ^::
+    ip_header_hop_limit h) ++
+  word128_to_bytes (ip_header_src_address h) ++
+  word128_to_bytes (ip_header_dst_address h).
 
-  Inductive ip_throughput :=
-  | IpThroughputNormal
-  | IpThroughputHigh.
+Definition bytes_to_ip_header (bs : bytes) : option (ip_header * bytes) :=
+  match bytes_to_word32s bs with
+  | v_tc_fl :: pl_nh_hl ::
+    sa1 :: sa2 :: sa3 :: sa4 ::
+    da1 :: da2 :: da3 :: da4 :: ws' =>
+    let v := split1 4 _ v_tc_fl in
+    let tc_fl := split2 4 _ v_tc_fl in
+    let tc := split1 8 _ tc_fl in
+    let fl := split2 8 _ tc_fl in
+    let pl := split1 16 _ pl_nh_hl in
+    let nh_hl := split2 16 _ pl_nh_hl in
+    let nh' := split1 8 _ nh_hl in
+    let hl := split2 8 _ nh_hl in
+    let sa := (sa1 ^:: sa2 ^:: sa3 ^:: sa4)%word in
+    let da := (da1 ^:: da2 ^:: da3 ^:: da4)%word in
+    match word_to_ip_next_header nh' with
+    | Some nh =>
+      Some (IpHeader v tc fl pl nh hl sa da, word32s_to_bytes ws')
+    | None => None
+    end
+  | _ => None
+  end.
 
-  Definition ip_throughput_to_nat (t : ip_throughput) :=
-    match t with
-    | IpThroughputNormal => 0
-    | IpThroughputHigh => 1
-    end.
+Definition ip_datagram_to_bytes (d : ip_datagram) : bytes :=
+  ip_header_to_bytes (ip_datagram_header d) ++ (ip_datagram_payload d).
 
-  Definition ip_throughput_to_word (t : ip_throughput) : word 1 :=
-    natToWord _ (ip_throughput_to_nat t).
+Definition bytes_to_ip_datagram (bs : bytes) : option ip_datagram :=
+  match bytes_to_ip_header bs with
+  | Some (h, p) =>
+    if weqb $(length p) (ip_header_payload_length h) then Some (IpDatagram h p)
+    else None
+  | None => None
+  end.
 
-  Inductive ip_reliability :=
-  | IpReliabilityNormal
-  | IpReliabilityHigh.
+(* Component *)
+Definition ip_node := ip_address.
+Definition ip_message := bytes.
 
-  Definition ip_reliability_to_nat (r : ip_reliability) :=
-    match r with
-    | IpReliabilityNormal => 0
-    | IpReliabilityHigh => 1
-    end.
+Inductive ip_request :=
+| Send_ip
+  (tc : ip_traffic_class) (fl : ip_flow_label)
+  (nh : ip_next_header) (hl : ip_hop_limit)
+  (sa da : ip_address) (p : ip_payload).
 
-  Definition ip_reliability_to_word (r : ip_reliability) : word 1 :=
-    natToWord _ (ip_reliability_to_nat r).
+Inductive ip_indication :=
+| Receive_ip (d : ip_datagram).
 
-  Record ip_service_type :=
-    IpServiceType {
-      ip_service_type_precedence : ip_precedence;
-      ip_service_type_delay : ip_delay;
-      ip_service_type_throughput : ip_throughput;
-      ip_service_type_reliability : ip_reliability;
-    }.
+Section sub_interfaces.
 
-  Definition ip_service_type_to_word (st : ip_service_type) : word 8 :=
-    let p := ip_service_type_precedence st in
-    let pw := ip_precedence_to_word p in
-    let d := ip_service_type_delay st in
-    let dw := ip_delay_to_word d in
-    let t := ip_service_type_throughput st in
-    let tw := ip_throughput_to_word t in
-    let r := ip_service_type_reliability st in
-    let rw := ip_reliability_to_word r in
-    combine (wzero 2) (combine rw (combine tw (combine dw pw))).
+  Import VectorNotations.
 
-End ip.
+  Definition request_fl_ip : Type := request_fl ip_node ip_message.
+  Definition indication_fl_ip : Type := indication_fl ip_node ip_message.
+
+  Definition ip_sub_interfaces : interfaces :=
+    existT _ _ [(request_fl_ip, indication_fl_ip)].
+
+End sub_interfaces.
+
+Definition ip_state := unit.
+
+Definition ip :=
+  let initialize n := tt in
+  let request n s ir :=
+    match ir with
+    | Send_ip tc fl nh hl sa da p =>
+      let h := IpHeader ip_version_6 tc fl $(length p) nh hl sa da in
+      let d := IpDatagram h p in
+      let s' := s in
+      let ors := [Send_fl da (ip_datagram_to_bytes d)] in
+      let ois := [] in
+      (s', ors, ois)
+    end in
+  let indication n' s ii :=
+    match ii with
+    | Deliver_fl n m =>
+      match bytes_to_ip_datagram m with
+      | Some d =>
+        let s' := s in
+        let ors := [] in
+        let ois :=
+          if weqb n' (ip_header_dst_address (ip_datagram_header d)) then
+            [Receive_ip d]
+          else [] in
+        (s', ors, ois)
+      | None =>
+        let s' := s in
+        let ors := [] in
+        let ois := [] in
+        (s', ors, ois)
+      end
+    end in
+  let periodic n s :=
+    let s' := s in
+    let ors := [] in
+    let ois := [] in
+    (s', ors, ois) in
+  @Component ip_node ip_message ip_request ip_indication
+    ip_sub_interfaces ip_state
+    initialize request indication periodic.
+
+Definition ip_stack : stack ip_node ip_message (ir_event ip) (oi_event ip).
+Proof.
+  apply ComponentStack, TupleMapCons; [apply FairLossLink | apply TupleMapNil].
+Defined.
